Sketch of a complicated data structures with a lot of invariants... WIP

test/AssocList.fst
@@ -7,11 +7,173 @@ module M = FStar.Map
 module B = LowStar.Buffer
 module HS = FStar.HyperStack
 module ST = FStar.HyperStack.ST
+module LL1 = LowStar.Lib.LinkedList
+module LL2 = LowStar.Lib.LinkedList2
 
 open LowStar.BufferOps
 open FStar.HyperStack.ST
 
 #set-options "--fuel 0 --ifuel 0"
+
+// Simple representation of noise_handshake. One extra indirection compared to
+// wireguard, alas.
+let handshake_state = B.buffer UInt8.t
+
+noeq
+// Simplified equivalent of wg_peer.
+type peer = {
+  hs: handshake_state;
+  id: UInt64.t;
+  device: B.pointer device;
+}
+
+// Simplified equivalent of wg_device.
+and device = {
+  peers: LL2.t peer;
+  // I'm doing pointer sharing here so that the peers in peer_of_id are pointing
+  // directly to the list cells in the linked list, like in WireGuard
+  peer_of_id: I.t UInt64.t (LL1.t peer);
+  r: HS.rid;
+  r_peers: HS.rid;
+  r_peer_of_id: HS.rid;
+  r_handshake: HS.rid;
+}
+
+/// A single peer
+/// -------------
+let peer_invariant (h: HS.mem) (p: peer) =
+  B.live h p.hs /\ B.length p.hs == 8 /\
+  B.freeable p.hs
+
+let peer_footprint (h: HS.mem) (p: peer) =
+  B.loc_addr_of_buffer p.hs
+
+/// Properties of the payload of the linked list
+/// --------------------------------------------
+
+// Cannot use List.Tot.fold_right because GTot / Tot effect mistmatch
+let rec peers_footprint (h: HS.mem) (ps: list peer): GTot B.loc =
+  allow_inversion (list peer);
+  match ps with
+  | [] -> B.loc_none
+  | p :: ps -> peer_footprint h p `B.loc_union` peers_footprint h ps
+
+let rec peers_disjoint (h: HS.mem) (ps: list peer) =
+  allow_inversion (list peer);
+  match ps with
+  | [] -> True
+  | p :: ps ->
+      peer_footprint h p `B.loc_disjoint` peers_footprint h ps /\
+      peers_disjoint h ps
+
+let rec peers_invariant (h: HS.mem) (r: HS.rid) (ps: list peer) =
+  allow_inversion (list peer);
+  match ps with
+  | [] -> True
+  | p :: ps ->
+      B.(loc_region_only false r `loc_includes` peer_footprint h p) /\
+      peer_invariant h p /\
+      peers_disjoint h ps /\
+      peers_invariant h r ps
+
+// TODO: ids are pairwise disjoint, to facilitate insertion
+
+/// Relating peer_of_id to a given list of peers
+/// --------------------------------------------
+
+let rec peer_by_id (id: UInt64.t) (ps: list peer) =
+  allow_inversion (list peer);
+  match ps with
+  | p :: ps ->
+      if p.id = id then
+        Some p
+      else
+        peer_by_id id ps
+  | [] ->
+      None
+
+let peer_of_id_in_peers (h: HS.mem) (d: device) (i: UInt64.t) =
+  let m = I.v h d.peer_of_id in
+  let p = peer_by_id i (LL2.v h d.peers) in
+  match M.sel m i with
+  | None -> p == None
+  | Some ptr ->
+      ~(B.g_is_null ptr) /\
+      p == Some ((B.deref h ptr).LL1.data)
+
+/// Back pointers invariant
+/// -----------------------
+
+let rec peers_back (h: HS.mem) (d: device) (ps: list peer) =
+  allow_inversion (list peer);
+  match ps with
+  | p :: ps ->
+      B.deref h p.device == d /\
+      peers_back h d ps
+  | [] ->
+      True
+
+/// Global invariant on the device
+/// ------------------------------
+
+unfold
+let invariant (h: HS.mem) (d: device) =
+  ST.is_eternal_region d.r /\
+  ST.is_eternal_region d.r_peers /\
+  ST.is_eternal_region d.r_peer_of_id /\
+  ST.is_eternal_region d.r_handshake /\
+
+  HS.extends d.r_peers d.r /\
+  HS.extends d.r_peer_of_id d.r /\
+  HS.extends d.r_handshake d.r /\
+
+  HS.parent d.r_peers == d.r /\
+  HS.parent d.r_peer_of_id == d.r /\
+  HS.parent d.r_handshake == d.r /\
+
+  B.(loc_disjoint (loc_region_only false d.r_peers) (loc_region_only false d.r_peer_of_id)) /\
+  B.(loc_disjoint (loc_region_only false d.r_peers) (loc_region_only false d.r_handshake)) /\
+  B.(loc_disjoint (loc_region_only false d.r_peer_of_id) (loc_region_only false d.r_handshake)) /\
+
+  d.peers.LL2.r == d.r_peers /\
+  I.region_of d.peer_of_id == B.loc_all_regions_from false d.r_peer_of_id /\
+  // This is covered by the peers_invariant:
+  // loc_region d.r_handshake `loc_includes` peers_footprint (LL2.v h d.peers)
+
+  (forall (i: UInt64.t). {:pattern peer_of_id_in_peers h d i }
+    peer_of_id_in_peers h d i) /\
+  peers_back h d (LL2.v h d.peers) /\
+
+  LL2.invariant h d.peers /\
+  I.invariant h d.peer_of_id
+
+#push-options "--fuel 1"
+let create_in (r: HS.rid): ST device
+  (requires fun h0 ->
+    ST.is_eternal_region r)
+  (ensures fun h0 d h1 ->
+    invariant h1 d /\
+    B.(modifies loc_none h0 h1) /\
+    I.v h1 d.peer_of_id == M.const None /\
+    LL2.v h1 d.peers == [] /\
+    d.r == r)
+=
+  let r_peers = ST.new_region r in
+  let r_peer_of_id = ST.new_region r in
+  let r_handshake = ST.new_region r in
+  let peers = LL2.create_in r_peers in
+  let peer_of_id = I.create_in r_peer_of_id in
+  { peers; peer_of_id; r; r_peers; r_peer_of_id; r_handshake }
+#pop-options
+
+let test (): St unit =
+  let r = ST.new_region HS.root in
+  let d = create_in r in
+  // TODO: talk about where the backpoint lives (which region?), how live it is, etc. etc. etc.
+  let p = { id = 0UL; hs = B.malloc d.r_handshake 0uy 8ul; device = B.malloc HS.root d 1ul } in
+  LL2.push d.peers p;
+  let h1 = ST.get () in
+  () // assert (invariant h1 d)
 
 let main (): St Int32.t =
   let r = ST.new_region HS.root in
